Add WFAig equivalents of all aig modification methods

Valaig/Aig/WellFormed.lean
@@ -1,6 +1,6 @@
 module
 
-public import Valaig.Aig
+public import Valaig.Aig.Basic
 public import Valaig.Aig.Lemmas.WellFormed
 
 public section
@@ -29,6 +29,29 @@ theorem WF :
     aig.raw.WF :=
   aig.wf
 
+@[always_inline, inherit_doc Aig.setNext]
+def setNext (aig : WFAig) (idx : LatchIdx) (next : Lit) (valid : idx.validIn aig := by grind)
+    (nextValid : next.validIn aig := by grind) : WFAig :=
+  aig.raw.setNext idx next |>.toWF
+
+@[simp, grind =]
+theorem raw_setNext {idx : LatchIdx} {next : Lit} valid nextValid :
+    (aig.setNext idx next valid nextValid).raw = aig.raw.setNext idx next := by
+  rfl
+
+@[always_inline, inherit_doc Aig.setReset]
+def setReset (aig : WFAig) (idx : LatchIdx) (reset : Option Lit) (valid : idx.validIn aig := by grind)
+    (resetValid :
+      match reset with
+      | none => True
+      | some lit => lit.var < idx.getVar aig := by grind) : WFAig :=
+  aig.raw.setReset idx reset |>.toWF
+
+@[simp, grind =]
+theorem raw_setReset {idx : LatchIdx} {reset : Option Lit} valid resetValid :
+    (aig.setReset idx reset valid resetValid).raw = aig.raw.setReset idx reset := by
+  rfl
+
 @[always_inline, inherit_doc Aig.addInput]
 def addInput (aig : WFAig) : WFAig × InputIdx :=
   let (eq:=_) (aig, idx) := aig.raw.addInput
@@ -50,8 +73,7 @@ def addLatch (aig : WFAig) (next : Lit) (reset : Option Lit := none)
     (resetValid :
         match reset with
         | none => True
-        | some lit => lit.validIn aig := by grind) :
-    WFAig × LatchIdx :=
+        | some lit => lit.validIn aig := by grind) : WFAig × LatchIdx :=
   let (eq:=_) (aig, idx) := aig.raw.addLatch next reset
   (aig.toWF, idx)
 
@@ -97,6 +119,150 @@ theorem raw_fst_addAnd {lhs rhs : Lit} lvalid rvalid :
 @[simp, grind =]
 theorem snd_addAnd {lhs rhs : Lit} lvalid rvalid :
     (aig.addAnd lhs rhs lvalid rvalid).snd = (aig.raw.addAnd lhs rhs).snd := by
+  rfl
+
+@[always_inline, inherit_doc Aig.inputToLatch]
+def inputToLatch (aig : WFAig) (idx : InputIdx) (next : Lit) (reset : Option Lit := none)
+    (valid : idx.validIn aig := by grind)
+    (varValid : (idx.getVar aig).validIn aig := by grind)
+    (nextValid : next.validIn aig := by grind)
+    (resetValid :
+      match reset with
+      | none => True
+      | some lit => lit.var < idx.getVar aig := by grind) : WFAig × LatchIdx :=
+  let (eq:=_) (aig, latch) := aig.raw.inputToLatch idx next reset
+  (aig.toWF, latch)
+
+@[simp, grind =]
+theorem raw_fst_inputToLatch {idx : InputIdx} {next : Lit} {reset : Option Lit} valid varValid nextValid resetValid :
+    (aig.inputToLatch idx next reset valid varValid nextValid resetValid).fst.raw =
+    (aig.raw.inputToLatch idx next reset).fst := by
+  rfl
+
+@[simp, grind =]
+theorem snd_inputToLatch {idx : InputIdx} {next : Lit} {reset : Option Lit} valid varValid nextValid resetValid :
+    (aig.inputToLatch idx next reset valid varValid nextValid resetValid).snd = (aig.raw.inputToLatch idx next reset).snd := by
+  rfl
+
+@[always_inline, inherit_doc Aig.inputToAnd]
+def inputToAnd (aig : WFAig) (idx : InputIdx) (lhs rhs : Lit)
+    (valid : idx.validIn aig := by grind)
+    (varValid : (idx.getVar aig).validIn aig := by grind)
+    (lvalid : lhs.var < idx.getVar aig := by grind)
+    (rvalid : rhs.var < idx.getVar aig := by grind) : WFAig :=
+  aig.raw.inputToAnd idx lhs rhs |>.toWF
+
+@[simp, grind =]
+theorem raw_inputToAnd {idx : InputIdx} {lhs rhs : Lit} valid varValid lvalid rvalid :
+    (aig.inputToAnd idx lhs rhs valid varValid lvalid rvalid).raw = aig.raw.inputToAnd idx lhs rhs:= by
+  rfl
+
+@[always_inline, inherit_doc Aig.changeInputIdx]
+def changeInputIdx (aig : WFAig) (old new : InputIdx)
+    (valid : old.validIn aig := by grind)
+    (varValid : (old.getVar aig).validIn aig := by grind)
+    (unused : ¬new.validIn aig ∨ old = new := by grind) : WFAig :=
+  aig.raw.changeInputIdx old new |>.toWF
+
+@[simp, grind =]
+theorem raw_changeInputIdx {old new : InputIdx} valid varValid unused :
+    (aig.changeInputIdx old new valid varValid unused).raw = aig.raw.changeInputIdx old new := by
+  rfl
+
+@[always_inline, inherit_doc Aig.latchToInput]
+def latchToInput (aig : WFAig) (idx : LatchIdx)
+    (valid : idx.validIn aig := by grind)
+    (varValid : (idx.getVar aig).validIn aig := by grind) : WFAig × InputIdx :=
+  let (eq:=_) (aig, idx) := aig.raw.latchToInput idx
+  (aig.toWF, idx)
+
+@[simp, grind =]
+theorem raw_fst_latchToInput {idx : LatchIdx} valid varValid :
+    (aig.latchToInput idx valid varValid).fst.raw = (aig.raw.latchToInput idx).fst := by
+  rfl
+
+@[simp, grind =]
+theorem snd_latchToInput {idx : LatchIdx} valid varValid :
+    (aig.latchToInput idx valid varValid).snd = (aig.raw.latchToInput idx).snd := by
+  rfl
+
+@[always_inline, inherit_doc Aig.latchToAnd]
+def latchToAnd (aig : WFAig) (idx : LatchIdx) (lhs rhs : Lit)
+    (valid : idx.validIn aig := by grind)
+    (varValid : (idx.getVar aig).validIn aig := by grind)
+    (lvalid : lhs.var < idx.getVar aig := by grind)
+    (rvalid : rhs.var < idx.getVar aig := by grind) : WFAig :=
+  aig.raw.latchToAnd idx lhs rhs |>.toWF
+
+@[simp, grind =]
+theorem raw_latchToAnd {idx : LatchIdx} {lhs rhs : Lit} valid varValid lvalid rvalid :
+    (aig.latchToAnd idx lhs rhs valid varValid lvalid rvalid).raw = aig.raw.latchToAnd idx lhs rhs:= by
+  rfl
+
+@[always_inline, inherit_doc Aig.changeLatchIdx]
+def changeLatchIdx (aig : WFAig) (old new : LatchIdx)
+    (valid : old.validIn aig := by grind)
+    (varValid : (old.getVar aig).validIn aig := by grind)
+    (unused : ¬new.validIn aig ∨ old = new := by grind) : WFAig :=
+  aig.raw.changeLatchIdx old new |>.toWF
+
+@[simp, grind =]
+theorem raw_changeLatchIdx {old new : LatchIdx} valid varValid unused :
+    (aig.changeLatchIdx old new valid varValid unused).raw = aig.raw.changeLatchIdx old new := by
+  rfl
+
+@[always_inline, inherit_doc Aig.andToInput]
+def andToInput (aig : WFAig) (var : Var)
+    (valid : var.validIn aig := by grind)
+    (isAnd : aig.raw[var] matches .and _ _ := by grind) : WFAig × InputIdx :=
+  let (eq:=_) (aig, idx) := aig.raw.andToInput var
+  (aig.toWF, idx)
+
+@[simp, grind =]
+theorem raw_fst_andToInput {var : Var} valid isAnd :
+    (aig.andToInput var valid isAnd).fst.raw = (aig.raw.andToInput var).fst := by
+  rfl
+
+@[simp, grind =]
+theorem snd_andToInput {var : Var} valid isAnd :
+    (aig.andToInput var valid isAnd).snd = (aig.raw.andToInput var).snd := by
+  rfl
+
+@[always_inline, inherit_doc Aig.andToLatch]
+def andToLatch (aig : WFAig) (var : Var) (next : Lit) (reset : Option Lit)
+    (valid : var.validIn aig := by grind)
+    (nextValid : next.validIn aig := by grind)
+    (resetValid :
+        match reset with
+        | none => True
+        | some lit => lit.var < var := by grind)
+    (isAnd : aig.raw[var] matches .and _ _ := by grind) : WFAig × LatchIdx :=
+  let (eq:=_) (aig, idx) := aig.raw.andToLatch var next reset
+  (aig.toWF, idx)
+
+@[simp, grind =]
+theorem raw_fst_andToLatch {var : Var} {next : Lit} {reset : Option Lit} valid nextValid resetValid isAnd :
+    (aig.andToLatch var next reset valid nextValid resetValid isAnd).fst.raw =
+    (aig.raw.andToLatch var next reset).fst := by
+  rfl
+
+@[simp, grind =]
+theorem snd_andToLatch {var : Var} {next : Lit} {reset : Option Lit} valid nextValid resetValid isAnd :
+    (aig.andToLatch var next reset valid nextValid resetValid isAnd).snd =
+    (aig.raw.andToLatch var next reset).snd := by
+  rfl
+
+@[inline]
+def rewriteAnd (aig : WFAig) (var : Var) (lhs rhs : Lit)
+    (valid : var.validIn aig := by grind)
+    (isAnd : aig.raw[var] matches .and _ _ := by grind)
+    (lvalid : lhs.var < var := by grind)
+    (rvalid : rhs.var < var := by grind) : WFAig :=
+  aig.raw.rewriteAnd var lhs rhs |>.toWF
+
+@[simp, grind =]
+theorem raw_rewriteAnd {var : Var} {lhs rhs : Lit} valid isAnd lvalid rvalid :
+    (aig.rewriteAnd var lhs rhs valid isAnd lvalid rvalid).raw = aig.raw.rewriteAnd var lhs rhs := by
   rfl
 
 end Valaig.WFAig
