Valaig/Aig.lean
@@ -2,5 +2,6 @@ module
 
 public import Valaig.Aig.Basic
 public import Valaig.Aig.Lemmas
+public import Valaig.Aig.WellFormed
 public import Valaig.Aig.CheckWellFormed
 public import Valaig.Aig.Walker
